src/Parsers/BooleanRecognizer.v
@@ -1,8 +1,8 @@
 (** * Definition of a boolean-returning CFG parser-recognizer *)
 Require Import Omega.
 Require Import Coq.Lists.List Coq.Program.Program Coq.Program.Wf Coq.Arith.Wf_nat Coq.Arith.Compare_dec Coq.Classes.RelationClasses Coq.Strings.String.
-Require Import Parsers.ContextFreeGrammar Parsers.Specification Parsers.ContextFreeGrammarNotations.
-Require Import Common Common.ilist Common.Wf.
+Require Import Parsers.ContextFreeGrammar Parsers.ContextFreeGrammarNotations.
+Require Import Common Common.Wf.
 
 Set Implicit Arguments.
 Local Open Scope string_like_scope.
@@ -32,9 +32,6 @@ Section recursive_descent_parser.
 
     Section parts.
       Section item.
-        (** We require that the list of names be non-empty; we
-            do this by passing the first element separately, rather
-            than invoking dependent types and proofs. *)
         Context (str : StringWithSplitState String split_stateT)
                 (str_matches_name : string -> bool).
 
