src/Parsers/ContextFreeGrammar.v
@@ -42,7 +42,6 @@ Section cfg.
 
     (** A [grammar] consists of [productions] to match a string
         against, and a function mapping names to [productions]. *)
-    (** TODO(jgross): also include list of valid starting non-terminals, for convenience and notation *)
     (** TODO(jgross): look up notations for specifying these nicely *)
     Record grammar :=
       {
